Poor Person's Verified Totalizer Encoding
Fixed the definitions and completed the general proof of
correctness. Still not wired to the VEncCNF framework.

Experiments/Totalizer.lean
@@ -1,11 +1,20 @@
 import Trestle.Encode.Cardinality.Defs
 import Trestle.Solver.Dimacs
 
+namespace List
+
+-- By Kenny Lau
+-- https://leanprover.zulipchat.com/#narrow/channel/217875-Is-there-code-for-X.3F/topic/List.20length.20induction/near/554091009
+theorem length_wf {α : Type} : WellFounded (λ (x y : List α) ↦ x.length < y.length) := InvImage.wf _ Nat.lt_wfRel.2
+
+def length_induction {α : Type} := @WellFounded.induction (List α) _ length_wf
+
+end List
+
 namespace Trestle.Encode.Cardinality
 
 open EncCNF Model PropFun
 
--- NOTE: Maybe return a Vector of ν so that one can use Literal.{pos,neg} directly.
 def totalizer [LE ν] [DecidableLE ν] [HAdd ν ℕ ν] {k : ℕ} (c : Vector (Literal ν) k) (nextVar : ν) : Array (Clause (Literal ν)) × Vector (Literal ν) k × Option ν :=
 match h:c with
 | Vector.mk carr _ => match carr with
@@ -16,20 +25,12 @@ match h:c with
       let ltot := totalizer (@Vector.mk (Literal ν) ((x :: (y :: t)).length / 2) ⟨(x :: (y :: t)).take ((x :: (y :: t)).length / 2)⟩ (by simp; omega)) (nextVar + c.size);
       let rtot := totalizer (@Vector.mk (Literal ν) ((x :: (y :: t)).length - (x :: (y :: t)).length / 2) ⟨(x :: (y :: t)).drop ((x :: (y :: t)).length / 2)⟩ (by simp)) (Option.getD ltot.snd.snd (nextVar + c.size));
       let newVars := List.map (λ n ↦ nextVar + n) (List.range c.size);
-      -- FIXME These folds/mapFinIdxs should be restructured to 1) either use concat or flatten but not both and 2) merge consecutive mapFnIdxs
-  ⟨ltot.fst ++ rtot.fst ++ ⟨(List.foldl List.concat (List.mapFinIdx ltot.snd.fst.toList (λ i _ ilt ↦ #[LitVar.negate (ltot.snd.fst.toList.get ⟨i, ilt⟩), Literal.pos (newVars.get ⟨i, by next klen _ => simp [← Array.length_toList] at klen; simp [newVars, h, Vector.size, ← klen]; simp [ltot] at ilt; trans (t.length + 1 + 1) / 2; assumption; omega⟩)])) []) ++ List.flatten (List.mapFinIdx ltot.snd.fst.toList (λ i _ ilt ↦ (List.mapFinIdx rtot.snd.fst.toList (λ j _ jlt ↦ #[LitVar.negate (rtot.snd.fst.toList.get ⟨j, jlt⟩), Literal.pos (newVars.get ⟨j, by next klen _ _ => simp [← Array.length_toList] at klen; simp [newVars, h, Vector.size, ← klen]; simp [rtot] at jlt; trans t.length + 1 + 1 - (t.length + 1 + 1) / 2; assumption; simp⟩)])) ++ (List.mapFinIdx rtot.snd.fst.toList (λ j _ jlt ↦ #[LitVar.negate (ltot.snd.fst.toList.get ⟨i, ilt⟩), LitVar.negate (rtot.snd.fst.toList.get ⟨j, jlt⟩), Literal.pos (newVars.get ⟨(i + j).succ, by next klen _ _ => simp [newVars, h, Vector.size, ← klen]; simp [ltot] at ilt; simp [rtot] at jlt; rw [Nat.sub_add_comm, Nat.lt_iff_le_pred] at jlt; simp at jlt; have ijlt := Nat.add_lt_add_of_lt_of_le ilt jlt; rw [← Nat.add_sub_assoc] at ijlt; simp at ijlt; exact ijlt; omega; omega; omega⟩)]))))⟩ ++ ⟨List.foldl List.concat (List.mapFinIdx ltot.snd.fst.toList (λ i _ ilt ↦ #[Literal.neg (newVars.get ⟨i + rtot.snd.fst.size, by next klen _ => simp +arith [newVars, h, Vector.size, ← klen]; rw [← Nat.add_sub_assoc, Nat.sub_le_iff_le_add]; simp +arith [ltot] at ilt ⊢; assumption; omega⟩), ltot.snd.fst.toList.get ⟨i, ilt⟩])) [] ++ List.flatten (List.mapFinIdx ltot.snd.fst.toList (λ i _ ilt ↦ (List.mapFinIdx rtot.snd.fst.toList (λ j _ jlt ↦ #[Literal.neg (newVars.get ⟨j + ltot.snd.fst.size, by next klen _ _ => simp +arith [newVars, h, Vector.size, ← klen]; simp +arith [ltot, Nat.lt_sub_iff_add_lt] at jlt; assumption⟩), rtot.snd.fst.toList.get ⟨j, jlt⟩])) ++ (List.mapFinIdx rtot.snd.fst.toList (λ j _ jlt ↦ #[Literal.neg (newVars.get ⟨i + j, by next klen _ _ => simp [newVars, h, Vector.size, ← klen]; simp +arith [ltot] at ilt; simp +arith [rtot] at jlt; have ijlt := Nat.add_lt_add_of_le_of_lt ilt jlt; rw [← Nat.add_sub_assoc, Nat.add_sub_cancel_left] at ijlt; trans t.length + 1; assumption; simp; omega⟩), ltot.snd.fst.toList.get ⟨i, ilt⟩, rtot.snd.fst.toList.get ⟨j, jlt⟩]))))⟩, ⟨@Vector.mk _ c.size ⟨newVars⟩ (by simp [newVars, -List.pure_def, -List.bind_eq_flatMap, List.size_toArray]), Option.getD rtot.snd.snd (nextVar + c.size)⟩⟩
+  ⟨ltot.fst ++ rtot.fst
+++ ⟨List.flatten ((List.finRange ltot.snd.fst.size.succ).map (Fin.cases ((List.finRange rtot.snd.fst.size.succ).filterMap (Fin.cases none (λ j ↦ some #[LitVar.negate (rtot.snd.fst.get j), Literal.pos (newVars.get ⟨j.val, by next klen => simp [← Array.length_toList] at klen; simp [newVars, h, Vector.size, ← klen]; have jlt := j.prop; simp only [rtot] at jlt; trans t.length + 1 + 1 - (t.length + 1 + 1) / 2; assumption; simp⟩)]))) (λ i ↦ (List.finRange rtot.snd.fst.size.succ).map (Fin.cases (#[LitVar.negate (ltot.snd.fst.get i), Literal.pos (newVars.get ⟨i.val, by next klen => simp [← Array.length_toList] at klen; simp [newVars, h, Vector.size, ← klen]; have ilt := i.prop; simp [-Fin.is_lt, ltot] at ilt; trans (t.length + 1 + 1) / 2; assumption; omega⟩)]) (λ j ↦ #[LitVar.negate (ltot.snd.fst.get i), LitVar.negate (rtot.snd.fst.get j), Literal.pos (newVars.get ⟨(i.val + j.val).succ, by next klen => simp [newVars, h, Vector.size, ← klen]; have ilt := i.prop; simp [-Fin.is_lt, ltot, Vector.size] at ilt; have jlt := j.prop; simp [-Fin.is_lt, Vector.size, rtot] at jlt; rw [Nat.lt_iff_le_pred] at jlt; have ijlt := Nat.add_lt_add_of_lt_of_le ilt jlt; rw [← Nat.add_sub_assoc] at ijlt; simp +arith at ijlt; rw [← Nat.add_sub_assoc, Nat.add_sub_cancel_left] at ijlt; exact ijlt; omega; omega; omega⟩)])))))⟩
+++ ⟨List.flatten ((List.finRange ltot.snd.fst.size.succ).map (Fin.cases ((List.finRange rtot.snd.fst.size.succ).filterMap (Fin.cases none (λ j ↦ some #[rtot.snd.fst.get j, Literal.neg (newVars.get ⟨j.val + ltot.snd.fst.size, by next klen => simp +arith [newVars, h, Vector.size, ← klen]; have jlt := j.prop; simp +arith [ltot, Nat.lt_sub_iff_add_lt] at jlt; assumption⟩)]))) (λ i ↦ (List.finRange rtot.snd.fst.size.succ).map (Fin.cases (#[ltot.snd.fst.get i, Literal.neg (newVars.get ⟨i.val + rtot.snd.fst.size, by next klen => simp +arith [newVars, h, Vector.size, ← klen]; rw [← Nat.add_sub_assoc, Nat.sub_le_iff_le_add]; have ilt := i.prop; simp +arith [Vector.size, ltot] at ilt ⊢; assumption; omega⟩)]) (λ j ↦ #[ltot.snd.fst.get i, rtot.snd.fst.get j, Literal.neg (newVars.get ⟨i.val + j.val, by next klen => simp [newVars, h, Vector.size, ← klen]; have ilt := i.prop; simp +arith [Vector.size, ltot] at ilt; have jlt := j.prop; simp +arith [Vector.size, rtot] at jlt; have ijlt := Nat.add_lt_add_of_le_of_lt ilt jlt; rw [← Nat.add_sub_assoc, Nat.add_sub_cancel_left] at ijlt; trans t.length + 1; assumption; simp; omega⟩)])))))⟩
+, ⟨@Vector.mk _ c.size ⟨newVars⟩ (by simp [newVars, -List.pure_def, -List.bind_eq_flatMap, List.size_toArray]), Option.getD rtot.snd.snd (nextVar + c.size)⟩⟩
 termination_by c.size
 decreasing_by
-next klen =>
-  simp [h, Vector.size, ← klen]
-  omega
-next klen =>
-  simp [h, Vector.size, ← klen]
-next klen =>
-  simp [h, Vector.size, ← klen]
-  omega
-next klen =>
-  simp [h, Vector.size, ← klen]
 next klen =>
   simp [h, Vector.size, ← klen]
   omega
@@ -40,38 +41,20 @@ next absurd _ _ _ =>
   cases t with
   | nil => simp +arith at absurd
   | cons h t' => simp +arith at absurd
-next klen =>
-  simp [h, Vector.size, ← klen]
-  omega
-next klen =>
-  simp [h, Vector.size, ← klen]
-  omega
-next klen =>
-  simp [Vector.size, ← klen]
-  omega
-next klen =>
-  simp [Vector.size, ← klen]
-  omega
-next klen =>
-  simp [Vector.size, ← klen]
-  omega
-next klen =>
-  simp [Vector.size, ← klen]
-  omega
-next klen =>
-  simp [Vector.size, ← klen]
-  omega
-next klen =>
-  simp [Vector.size, ← klen]
-  omega
-next klen =>
-  simp [Vector.size, ← klen]
-next klen =>
-  simp [Vector.size, ← klen]
-next klen =>
-  simp [Vector.size, ← klen]
-next klen =>
-  simp [Vector.size, ← klen]
+next absurd _ _ _ =>
+  simp +arith [Nat.le_div_iff_mul_le] at absurd
+next absurd _ _ _ =>
+  simp +arith [Nat.lt_div_iff_mul_lt] at absurd
+  cases t with
+  | nil => simp +arith at absurd
+  | cons h t' => simp +arith at absurd
+next absurd _ _ _ =>
+  simp +arith [Nat.sub_eq_zero_iff_le, Nat.le_div_iff_mul_le] at absurd
+next absurd _ _ _ =>
+  simp +arith [Nat.lt_div_iff_mul_lt] at absurd
+  cases t with
+  | nil => simp +arith at absurd
+  | cons h t' => simp +arith at absurd
 
 -- #eval totalizer (@Vector.mk (Literal ℕ) 0 #[] (by simp)) 1
 -- #eval totalizer (@Vector.mk (Literal ℕ) 1 #[Literal.pos 1] (by simp)) 2
@@ -86,9 +69,7 @@ lemma totalizer_works1 : ∀ τ (a : Literal IVar) (m : IVar), let tot := totali
 lemma totalizer_works2 : ∀ (τ : PropAssignment IVar) (a b : Literal IVar) (m : IVar), let tot := totalizer (@Vector.mk (Literal IVar) 2 #[a, b] (by simp)) m; (∀ c ∈ tot.fst, ∃ l ∈ c, eval τ l) → tot.snd.fst.map (λ (l : Literal IVar) ↦ eval τ l) = ⟨Array.replicate (card (Multiset.ofList [a, b]) τ) true ++ Array.replicate (2 - card (Multiset.ofList [a,b]) τ) false, by simp; rw [← Nat.add_sub_assoc]; simp; split <;> split <;> simp⟩ := by
   simp [totalizer, Vector.size]
   intros τ a b m sat
-  -- NOTE: How come I have to do this in 2 steps?
-  unfold totalizer at sat
-  simp at sat
+  simp [Fin.exists_fin_succ] at sat
   split
   next atrue =>
     simp [SemanticEntails.entails, satisfies] at atrue
@@ -105,12 +86,12 @@ lemma totalizer_works2 : ∀ (τ : PropAssignment IVar) (a b : Literal IVar) (m 
     next bfalse =>
       simp [SemanticEntails.entails, satisfies] at bfalse
       simp [List.range, List.range.loop]
-      have m1 := sat #[LitVar.mkNeg (m + 1), b]
+      have m1 := sat #[b, LitVar.mkNeg (m + 1)]
       simp [atrue, bfalse] at m1
       tauto
   next afalse =>
     simp [SemanticEntails.entails, satisfies] at afalse
-    have m1 := sat #[LitVar.mkNeg (m + 1), a]
+    have m1 := sat #[a, LitVar.mkNeg (m + 1)]
     simp [afalse] at m1
     split
     next btrue =>
@@ -122,11 +103,314 @@ lemma totalizer_works2 : ∀ (τ : PropAssignment IVar) (a b : Literal IVar) (m 
     next bfalse =>
       simp [SemanticEntails.entails, satisfies] at bfalse
       simp [List.range, List.range.loop]
-      have m0 := sat #[LitVar.mkNeg (m + 0), a, b]
+      have m0 := sat #[a, b, LitVar.mkNeg (m + 0)]
       simp [afalse, bfalse] at m0
       tauto
 
+-- NOTE: How is this possibly missing?
+lemma pred_add : ∀ {a b : ℕ}, 0 < b → a + b.pred = (a + b).pred := by
+  intros a b
+  cases b <;> simp
+
+lemma split_sum : ∀ {A B c : ℕ}, c < A + B → A ≤ c → B ≤ c → ∃ a b, c = (a + b).succ ∧ a < A ∧ b < B := by
+  intros A B c cltAB Alec Blec
+  have Apos := Nat.lt_of_le_of_lt (Nat.add_le_add_left Blec A) (Nat.add_lt_add_left cltAB A)
+  simp at Apos
+  have cpos := Nat.lt_of_lt_of_le Apos Alec
+  use A.pred, (c.pred - A.pred)
+  rw [Nat.add_sub_cancel' (Nat.pred_le_pred Alec), Nat.sub_lt_iff_lt_add, Nat.succ_pred (Nat.ne_of_gt cpos)]
+  simp [-Nat.pred_eq_sub_one, Nat.pred_lt_self Apos, pred_add Apos]
+  apply Nat.pred_lt_pred (Nat.ne_of_gt cpos)
+  · rw [Nat.add_comm]
+    assumption
+  · apply Nat.pred_le_pred
+    assumption
+
+lemma split_sum' : ∀ {A B c : ℕ}, c < A + B → ∃ a b, a + b = c ∧ ((a ≤ A ∧ b < B) ∨ (a < A ∧ b ≤ B))  := by
+  intros A B c cltAB
+  cases Nat.decLt c (max A B) with
+  | isTrue cltmax =>
+    simp at cltmax
+    cases cltmax with
+    | inl cltA =>
+      use c, 0
+      simp [cltA]
+    | inr cleqB =>
+      use 0, c
+      simp [cleqB]
+  | isFalse cgtmax =>
+    simp at cgtmax
+    use A, (c - A)
+    simp [cgtmax.left, Nat.sub_lt_iff_lt_add]
+    rw [Nat.add_comm]
+    assumption
+
+lemma bounded_sum : ∀ {A B M N c : ℕ}, A + B ≤ c → c < M + N → A ≤ M → B ≤ N → ∃ a b, (A + a) + (B + b) = c ∧ (((A + a ≤ M) ∧ (B + b < N)) ∨ ((A + a < M) ∧ (B + b ≤ N))) := by
+  intros A B M N c cgeAB cltMN AleM BleN
+  rw [← Nat.sub_lt_sub_iff_right cgeAB, Nat.sub_add_eq (M + N), Nat.sub_add_comm AleM, Nat.add_sub_assoc BleN] at cltMN
+  obtain ⟨a, b, absum⟩ := split_sum' cltMN
+  use a, b
+  omega
+
+set_option maxHeartbeats 500000
+
+lemma totalizer_works : ∀ {k : ℕ} (τ : PropAssignment IVar) (l : Vector (Literal IVar) k) (m : IVar), let tot := totalizer l m; (∀ c ∈ tot.fst, ∃ l ∈ c, eval τ l) → tot.snd.fst.map (λ (l : Literal IVar) ↦ eval τ l) = ⟨Array.replicate (card (Multiset.ofList l.toArray.toList) τ) true ++ Array.replicate (k - card (Multiset.ofList l.toArray.toList) τ) false, by simp; rw [← Nat.add_sub_assoc]; simp; simp [card]; trans l.size; apply Vector.countP_le_size; simp⟩ := by
+  intros k τ v
+  cases v with
+  | mk a asize =>
+    cases a with
+    | mk l =>
+      induction l using List.length_induction generalizing k with
+      | h l ih =>
+          cases k with
+          | zero =>
+            simp at asize
+            simp [totalizer, asize, card]
+          | succ n =>
+            cases n with
+            | zero =>
+              simp at asize
+              rw [List.length_eq_one_iff] at asize
+              obtain ⟨x, ax⟩ := asize
+              simp [ax, totalizer, SemanticEntails.entails, satisfies]
+              split <;> simp
+              next _ => assumption
+              next h =>
+                simp at h
+                assumption
+            | succ m =>
+              intro mvar t sat
+              simp at asize
+              obtain ⟨x, ⟨xt, xl⟩⟩ := List.exists_cons_of_length_eq_add_one asize
+              simp [xl] at asize
+              obtain ⟨y, ⟨w, yl⟩⟩ := List.exists_cons_of_length_eq_add_one asize
+              simp [yl] at xl
+              simp [xl, t, totalizer, Vector.size, -List.pure_def, -List.bind_eq_flatMap, -card_cons]
+              simp at ih
+              simp [t, xl, totalizer, Vector.size, Fin.exists_fin_succ] at sat
+              have takeih := @ih (List.take ((w.length + 1 + 1) / 2) (x :: y :: w)) (by simp [xl]; omega) ((w.length + 1 + 1) / 2) (by simp; omega) (mvar + (m + 1 + 1)) (by intro c cmem; have csat := sat c; simp [cmem] at csat; assumption)
+              have dropih := @ih (List.drop ((w.length + 1 + 1) / 2) (x :: y :: w)) (by simp [xl]) (w.length + 1 + 1 - (w.length + 1 + 1) / 2) (by simp) ((totalizer (@Vector.mk (Literal IVar) ((w.length + 1 + 1) / 2) ⟨List.take ((w.length + 1 + 1) / 2) (x :: y :: w)⟩ (by simp; omega)) (mvar + (m + 1 + 1))).snd.snd.getD (mvar + (m + 1 + 1))) (by intro c cmem; have csat := sat c; simp [cmem] at csat; assumption)
+              apply List.ext_get
+              · simp +arith [-List.pure_def, -List.bind_eq_flatMap, card]
+                rw [← Nat.add_sub_assoc]
+                · simp
+                · apply Nat.le_trans List.countP_le_length
+                  simp [yl] at asize
+                  simp [asize]
+              · simp +arith [-List.pure_def, -List.bind_eq_flatMap, -card_cons]
+                intros k kle klt
+                rw [List.getElem_append]
+                have card_sum : card ↑(x :: y :: w) τ = card ↑(List.take ((w.length + 1 + 1) / 2) (x :: y :: w)) τ + card ↑(List.drop ((w.length + 1 + 1) / 2) (x :: y :: w)) τ := by
+                  suffices takedrop : x :: y :: w = List.take ((w.length + 1 + 1) / 2) (x :: y :: w) ++ List.drop ((w.length + 1 + 1) / 2) (x :: y :: w) by
+                    rw [takedrop, card_append]
+                    simp [-card_cons]
+                  simp
+                split
+                next kltcard =>
+                  simp [-card_cons, card_sum] at kltcard ⊢
+                  cases Nat.decLt k (max (card ↑(List.take ((w.length + 1 + 1) / 2) (x :: y :: w)) τ) (card ↑(List.drop ((w.length + 1 + 1) / 2) (x :: y :: w)) τ)) with
+                  | isTrue kor =>
+                    simp at kor
+                    cases kor with
+                    | inl kltleft =>
+                      have fit := sat #[-(totalizer (@Vector.mk _ ((w.length + 1 + 1) / 2) ⟨List.take ((w.length + 1 + 1) / 2) (x :: y :: w)⟩ (by simp; omega)) (mvar + (m + 1 + 1))).snd.fst.get ⟨k, by simp [card] at kltleft; have klt2 := Nat.lt_of_lt_of_le kltleft List.countP_le_length; simp at klt2; exact klt2.left⟩, LitVar.mkPos (mvar + k)]
+                      simp at fit
+                      rw [← Bool.not_eq_true, ← Decidable.imp_iff_not_or] at fit
+                      apply fit
+                      · right; right; left
+                        use (List.finRange (w.length + 1 + 1 - (w.length + 1 + 1) / 2 + 1)).map (λ i_1 ↦ Fin.cases #[-(totalizer (@Vector.mk _ ((w.length + 1 + 1) / 2) ⟨List.take ((w.length + 1 + 1) / 2) (x :: y :: w)⟩ (by simp; omega)) (mvar + (m + 1 + 1))).snd.fst.get ⟨k, by have klt2 := Nat.lt_of_lt_of_le kltleft List.countP_le_length; simp at klt2; exact klt2.left⟩, LitVar.mkPos (mvar + k)] (λ j ↦ #[-(totalizer (@Vector.mk _ ((w.length + 1 + 1) / 2) ⟨List.take ((w.length + 1 + 1) / 2) (x :: y :: w)⟩ (by simp; omega)) (mvar + (m + 1 + 1))).snd.fst.get ⟨k, by have klt2 := Nat.lt_of_lt_of_le kltleft List.countP_le_length; simp at klt2; exact klt2.left⟩, -(totalizer (@Vector.mk _ ((w.length + 1 + 1) - (w.length + 1 + 1) / 2) ⟨List.drop ((w.length + 1 + 1) / 2) (x :: y :: w)⟩ (by simp)) ((totalizer (@Vector.mk _ ((w.length + 1 + 1) / 2) ⟨List.take ((w.length + 1 + 1) / 2) (x :: y :: w)⟩ (by simp; omega)) (mvar + (m + 1 + 1))).snd.snd.getD (mvar + (m + 1 + 1)))).snd.fst.get j, LitVar.mkPos (mvar + (k + j.val + 1))]) i_1)
+                        simp
+                        apply And.intro
+                        · right
+                          use ⟨k, by have klt2 := Nat.lt_of_lt_of_le kltleft List.countP_le_length; simp at klt2; exact klt2.left⟩
+                          simp
+                        · use 0
+                          simp
+                      · have evalk := congr_arg (λ a ↦ Array.getD a k true) takeih
+                        simp [Array.getD] at evalk
+                        split at evalk <;> split at evalk
+                        next =>
+                          simp [Array.getElem_append] at evalk
+                          simp [Vector.get, evalk]
+                          exact kltleft
+                        next _ absurd =>
+                          rw [Nat.add_sub_cancel'] at absurd
+                          · contradiction
+                          · apply Nat.le_trans List.countP_le_length (by simp)
+                        next _ absurd =>
+                          rw [Nat.add_sub_cancel'] at absurd
+                          · contradiction
+                          · apply Nat.le_trans List.countP_le_length (by simp)
+                        next kge _ =>
+                          have absurd := Nat.lt_of_lt_of_le kltleft List.countP_le_length
+                          simp at absurd
+                          cases kge absurd.left
+                    | inr kltright =>
+                      -- TODO: Copy and adjust from above (or use wlog)
+                      sorry
+                  | isFalse kge =>
+                    simp at kge
+                    obtain ⟨i, j, ⟨kijsucc, ⟨iltleft, jltright⟩⟩⟩ := split_sum kltcard kge.left kge.right
+                    have fit := sat #[-(totalizer (@Vector.mk _ ((w.length + 1 + 1) / 2) ⟨List.take ((w.length + 1 + 1) / 2) (x :: y :: w)⟩ (by simp; omega)) (mvar + (m + 1 + 1))).snd.fst.get ⟨i, by simp [card] at iltleft; have klt2 := Nat.lt_of_lt_of_le iltleft List.countP_le_length; simp at klt2; exact klt2.left⟩, -(totalizer (@Vector.mk _ ((w.length + 1 + 1) - (w.length + 1 + 1) / 2) ⟨List.drop ((w.length + 1 + 1) / 2) (x :: y :: w)⟩ (by simp)) ((totalizer (@Vector.mk _ ((w.length + 1 + 1) / 2) ⟨List.take ((w.length + 1 + 1) / 2) (x :: y :: w)⟩ (by simp; omega)) (mvar + (m + 1 + 1))).snd.snd.getD (mvar + (m + 1 + 1)))).snd.fst.get ⟨j, by simp [card] at jltright; have klt2 := Nat.lt_of_lt_of_le jltright List.countP_le_length; simp at klt2; exact klt2⟩, LitVar.mkPos (mvar + (i + j + 1))]
+                    simp at fit
+                    simp [kijsucc]
+                    rw [← Bool.not_eq_true, ← Bool.not_eq_true, ← Decidable.imp_iff_not_or, ← Decidable.imp_iff_not_or] at fit
+                    apply fit
+                    · right; right; left
+                      use (List.finRange (w.length + 1 + 1 - (w.length + 1 + 1) / 2 + 1)).map (λ i_1 ↦ Fin.cases #[-(totalizer (@Vector.mk _ ((w.length + 1 + 1) / 2) ⟨List.take ((w.length + 1 + 1) / 2) (x :: y :: w)⟩ (by simp; omega)) (mvar + (m + 1 + 1))).snd.fst.get ⟨i, sorry⟩, LitVar.mkPos (mvar + i)] (λ j ↦ #[-(totalizer (@Vector.mk _ ((w.length + 1 + 1) / 2) ⟨List.take ((w.length + 1 + 1) / 2) (x :: y :: w)⟩ (by simp; omega)) (mvar + (m + 1 + 1))).snd.fst.get ⟨i, sorry⟩, -(totalizer (@Vector.mk _ ((w.length + 1 + 1) - (w.length + 1 + 1) / 2) ⟨List.drop ((w.length + 1 + 1) / 2) (x :: y :: w)⟩ (by simp)) ((totalizer (@Vector.mk _ ((w.length + 1 + 1) / 2) ⟨List.take ((w.length + 1 + 1) / 2) (x :: y :: w)⟩ (by simp; omega)) (mvar + (m + 1 + 1))).snd.snd.getD (mvar + (m + 1 + 1)))).snd.fst.get j, LitVar.mkPos (mvar + (i + j.val + 1))])
+                i_1)
+                      simp
+                      apply And.intro
+                      · right
+                        use ⟨i, sorry⟩
+                        simp
+                      · use (⟨j, sorry⟩ : Fin _).succ
+                        simp
+                    · have evalk := congr_arg (λ a ↦ Array.getD a i true) takeih
+                      simp [Array.getD] at evalk
+                      split at evalk <;> split at evalk
+                      next =>
+                        simp [Array.getElem_append] at evalk
+                        simp [Vector.get, evalk]
+                        exact iltleft
+                      next _ absurd =>
+                        rw [Nat.add_sub_cancel'] at absurd
+                        · contradiction
+                        · apply Nat.le_trans List.countP_le_length (by simp)
+                      next _ absurd =>
+                        rw [Nat.add_sub_cancel'] at absurd
+                        · contradiction
+                        · apply Nat.le_trans List.countP_le_length (by simp)
+                      next kge _ =>
+                        have absurd := Nat.lt_of_lt_of_le iltleft List.countP_le_length
+                        simp at absurd
+                        cases kge absurd.left
+                    · have evalk := congr_arg (λ a ↦ Array.getD a j true) dropih
+                      simp [Array.getD] at evalk
+                      split at evalk <;> split at evalk
+                      next =>
+                        simp [Array.getElem_append] at evalk
+                        simp [Vector.get, evalk]
+                        exact jltright
+                      next _ absurd =>
+                        rw [Nat.add_sub_cancel'] at absurd
+                        · contradiction
+                        · apply Nat.le_trans List.countP_le_length (by simp)
+                      next _ absurd =>
+                        rw [Nat.add_sub_cancel'] at absurd
+                        · contradiction
+                        · apply Nat.le_trans List.countP_le_length (by simp)
+                      next kge _ =>
+                        have absurd := Nat.lt_of_lt_of_le jltright List.countP_le_length
+                        simp at absurd
+                        cases kge absurd
+                next kgecard =>
+                  simp [-card_cons, card_sum] at kgecard ⊢
+                  have kltcase : ∀ {a b : ℕ}, k = a + b → (card (Multiset.ofList (List.take ((w.length + 1 + 1) / 2) (x :: y :: w))) τ) ≤ a → (card (Multiset.ofList (List.drop ((w.length + 1 + 1) / 2) (x :: y :: w))) τ) ≤ b → a < (totalizer (@Vector.mk _ ((w.length + 1 + 1) / 2) ⟨List.take ((w.length + 1 + 1) / 2) (x :: y :: w)⟩ (by simp; omega)) (mvar + (m + 1 + 1))).snd.fst.size → b < (totalizer (@Vector.mk _ ((w.length + 1 + 1) - (w.length + 1 + 1) / 2) ⟨List.drop ((w.length + 1 + 1) / 2) (x :: y :: w)⟩ (by simp)) ((totalizer (@Vector.mk _ ((w.length + 1 + 1) / 2) ⟨List.take ((w.length + 1 + 1) / 2) (x :: y :: w)⟩ (by simp; omega)) (mvar + (m + 1 + 1))).snd.snd.getD (mvar + (m + 1 + 1)))).snd.fst.size → τ (mvar + k) = false := by
+                    intro a b kadd alb blb aub bub
+                    simp [Vector.size] at aub bub
+                    have fit := sat #[(totalizer (@Vector.mk _ ((w.length + 1 + 1) / 2) ⟨List.take ((w.length + 1 + 1) / 2) (x :: y :: w)⟩ (by simp; omega)) (mvar + (m + 1 + 1))).snd.fst.get ⟨a, by apply Nat.lt_of_le_of_lt _ aub; simp +arith [kadd]⟩, (totalizer (@Vector.mk _ ((w.length + 1 + 1) - (w.length + 1 + 1) / 2) ⟨List.drop ((w.length + 1 + 1) / 2) (x :: y :: w)⟩ (by simp)) ((totalizer (@Vector.mk _ ((w.length + 1 + 1) / 2) ⟨List.take ((w.length + 1 + 1) / 2) (x :: y :: w)⟩ (by simp; omega)) (mvar + (m + 1 + 1))).snd.snd.getD (mvar + (m + 1 + 1)))).snd.fst.get ⟨b, by apply Nat.lt_of_le_of_lt _ bub; simp +arith [kadd]⟩, LitVar.mkNeg (mvar + (a + b))]
+                    simp [← kadd] at fit ⊢
+                    rw [← Bool.not_eq_false, ← Bool.not_eq_false, ← Decidable.imp_iff_not_or, ← Decidable.imp_iff_not_or] at fit
+                    apply fit
+                    · right; right; right
+                      use (List.finRange (w.length + 1 + 1 - (w.length + 1 + 1) / 2 + 1)).map (λ j ↦ Fin.cases #[(totalizer (@Vector.mk _ ((w.length + 1 + 1) / 2) ⟨List.take ((w.length + 1 + 1) / 2) (x :: y :: w)⟩ (by simp; omega)) (mvar + (m + 1 + 1))).snd.fst.get ⟨a, by apply Nat.lt_of_le_of_lt _ aub; simp +arith [kadd]⟩, LitVar.mkNeg (mvar + (a + (w.length + 1 + 1 - (w.length + 1 + 1) / 2)))] (λ j ↦  #[(totalizer (@Vector.mk _ ((w.length + 1 + 1) / 2) ⟨List.take ((w.length + 1 + 1) / 2) (x :: y :: w)⟩ (by simp; omega)) (mvar + (m + 1 + 1))).snd.fst.get ⟨a, by apply Nat.lt_of_le_of_lt _ aub; simp +arith [kadd]⟩, (totalizer (@Vector.mk _ ((w.length + 1 + 1) - (w.length + 1 + 1) / 2) ⟨List.drop ((w.length + 1 + 1) / 2) (x :: y :: w)⟩ (by simp)) ((totalizer (@Vector.mk _ ((w.length + 1 + 1) / 2) ⟨List.take ((w.length + 1 + 1) / 2) (x :: y :: w)⟩ (by simp; omega)) (mvar + (m + 1 + 1))).snd.snd.getD (mvar + (m + 1 + 1)))).snd.fst.get j, LitVar.mkNeg (mvar + (a + j.val))]) j)
+                      apply And.intro
+                      · right
+                        use ⟨a, by apply Nat.lt_of_le_of_lt _ aub; simp +arith [kadd]⟩
+                      · simp
+                        use (⟨b, by apply Nat.lt_of_le_of_lt _ bub; simp +arith [kadd]⟩ : Fin _).succ
+                        simp [kadd, ← Nat.add_assoc]
+                    · have evalk := congr_arg (λ x ↦ Array.getD x a true) takeih
+                      simp [Array.getD] at evalk
+                      split at evalk
+                      next cardlt =>
+                        simp [Array.getElem_append] at evalk
+                        rw [← Nat.add_sub_assoc] at evalk
+                        · simp [cardlt, ← Nat.not_le, alb] at evalk
+                          exact evalk
+                        · simp [-card_cons, card]
+                          trans ((x :: y :: w).take ((w.length + 1 + 1) / 2)).length
+                          apply List.countP_le_length
+                          simp
+                      next _ cardge =>
+                        rw [Nat.not_lt] at cardge
+                        have absurd : (w.length + 1 + 1) / 2 < (w.length + 1 + 1) / 2 := Nat.lt_of_le_of_lt (Nat.le_trans cardge (by simp +arith [kadd])) aub
+                        simp at absurd
+                    · have evalk := congr_arg (λ x ↦ Array.getD x b true) dropih
+                      simp [Array.getD] at evalk
+                      split at evalk
+                      next cardlt =>
+                        simp [cardlt, Array.getElem_append] at evalk
+                        rw [← Nat.add_sub_assoc] at evalk
+                        · simp [cardlt, ← Nat.not_le, blb] at evalk
+                          exact evalk
+                        · simp [-card_cons, card]
+                          trans ((x :: y :: w).drop ((w.length + 1 + 1) / 2)).length
+                          · apply List.countP_le_length
+                          · simp
+                      next _ cardge =>
+                        rw [Nat.not_lt] at cardge
+                        have absurd : w.length + 1 + 1 - (w.length + 1 + 1) / 2 < w.length + 1 + 1 - (w.length + 1 + 1) / 2 := Nat.lt_of_le_of_lt (Nat.le_trans cardge (by simp +arith [kadd])) bub
+                        simp at absurd
+                  have klttots : k < (totalizer (@Vector.mk _ ((w.length + 1 + 1) / 2) ⟨List.take ((w.length + 1 + 1) / 2) (x :: y :: w)⟩ (by simp; omega)) (mvar + (m + 1 + 1))).snd.fst.size + (totalizer (@Vector.mk _ ((w.length + 1 + 1) - (w.length + 1 + 1) / 2) ⟨List.drop ((w.length + 1 + 1) / 2) (x :: y :: w)⟩ (by simp)) ((totalizer (@Vector.mk _ ((w.length + 1 + 1) / 2) ⟨List.take ((w.length + 1 + 1) / 2) (x :: y :: w)⟩ (by simp; omega)) (mvar + (m + 1 + 1))).snd.snd.getD (mvar + (m + 1 + 1)))).snd.fst.size := by
+                    simp +arith [yl] at asize
+                    simp +arith [asize, Vector.size]
+                    rw [← Nat.add_sub_assoc]
+                    · simpa
+                    . omega
+                  obtain ⟨i, j, ⟨kij, ijbounds⟩⟩ := bounded_sum kgecard klttots (by simp [-card_cons,card, Vector.size]; trans ((x :: y :: w).take ((w.length + 1 + 1) / 2)).length; apply List.countP_le_length; simp) (by simp [-card_cons,card, Vector.size]; trans ((x :: y :: w).drop ((w.length + 1 + 1) / 2)).length; apply List.countP_le_length; simp)
+                  cases ijbounds with
+                  | inl ilejlt =>
+                    rw [Nat.le_iff_lt_or_eq] at ilejlt
+                    cases ilejlt.left with
+                    | inl ilt =>
+                      apply kltcase kij.symm
+                      · simp
+                      · simp
+                      · assumption
+                      · exact ilejlt.right
+                    | inr ieq =>
+                      -- NOTE: Perhaps it makes sense to use (w.length ...) / 2 here directly instead of (totalizer ...).snd.fst.size?
+                      have fit := sat #[(totalizer (@Vector.mk _ ((w.length + 1 + 1) - (w.length + 1 + 1) / 2) ⟨List.drop ((w.length + 1 + 1) / 2) (x :: y :: w)⟩ (by simp)) ((totalizer (@Vector.mk _ ((w.length + 1 + 1) / 2) ⟨List.take ((w.length + 1 + 1) / 2) (x :: y :: w)⟩ (by simp; omega)) (mvar + (m + 1 + 1))).snd.snd.getD (mvar + (m + 1 + 1)))).snd.fst.get ⟨card (Multiset.ofList (List.drop ((w.length + 1 + 1) / 2) (x :: y :: w))) τ + j, ilejlt.right⟩, LitVar.mkNeg (mvar + (card (Multiset.ofList (List.drop ((w.length + 1 + 1) / 2) (x :: y :: w))) τ + j + (totalizer (@Vector.mk _ ((w.length + 1 + 1) / 2) ⟨List.take ((w.length + 1 + 1) / 2) (x :: y :: w)⟩ (by simp; omega)) (mvar + (m + 1 + 1))).snd.fst.size))]
+                      rw [Nat.add_comm] at kij
+                      simp [← kij, ieq, Vector.size] at fit ⊢
+                      rw [← Bool.not_eq_false, ← Decidable.imp_iff_not_or] at fit
+                      apply fit
+                      · right; right; right
+                        use (List.finRange (w.length + 1 + 1 - (w.length + 1 + 1) / 2 + 1)).filterMap (λ i ↦ Fin.cases none (λ j ↦ some #[(totalizer (@Vector.mk _ ((w.length + 1 + 1) - (w.length + 1 + 1) / 2) ⟨List.drop ((w.length + 1 + 1) / 2) (x :: y :: w)⟩ (by simp)) ((totalizer (@Vector.mk _ ((w.length + 1 + 1) / 2) ⟨List.take ((w.length + 1 + 1) / 2) (x :: y :: w)⟩ (by simp; omega)) (mvar + (m + 1 + 1))).snd.snd.getD (mvar + (m + 1 + 1)))).snd.fst.get j, LitVar.mkNeg (mvar + (j.val + (w.length + 1 + 1) / 2))]) i)
+                        simp
+                        use (⟨card (Multiset.ofList (List.drop ((w.length + 1 + 1) / 2) (x :: y :: w))) τ + j, by simp [Vector.size] at ilejlt; exact ilejlt.right⟩ : Fin _).succ
+                        simp
+                      · have evalk := congr_arg (λ z ↦ Array.getD z (card (Multiset.ofList (List.drop ((w.length + 1 + 1) / 2) (x :: y :: w))) τ + j) true) dropih
+                        simp [-add_lt_add_iff_left, -Nat.add_lt_add_iff_left, Array.getD] at evalk
+                        split at evalk
+                        next cardlt =>
+                          rw [← Nat.add_sub_assoc] at evalk
+                          · simp [cardlt, ← Nat.not_le] at evalk
+                            exact evalk
+                          · simp [-card_cons, card]
+                            trans ((x :: y :: w).drop ((w.length + 1 + 1) / 2)).length
+                            · apply List.countP_le_length
+                            · simp
+                        next _ cardge =>
+                          rw [Nat.not_lt] at cardge
+                          have absurd : w.length + 1 + 1 - (w.length + 1 + 1) / 2 < w.length + 1 + 1 - (w.length + 1 + 1) / 2 := Nat.lt_of_le_of_lt (Nat.le_trans cardge (by simp +arith [kij])) ilejlt.right
+                          simp at absurd
+                  | inr iltjle =>
+                    simp_rw [Nat.le_iff_lt_or_eq] at iltjle
+                    cases iltjle.right with
+                    | inl jlt =>
+                      apply kltcase kij.symm
+                      · simp
+                      · simp
+                      · exact iltjle.left
+                      · assumption
+                    | inr ieq =>
+                      sorry
+
 #eval Solver.Dimacs.printRichCnf IO.print ((((LawfulState.new ⟨5, by simp⟩ ⟨λ u : Fin 3 ↦ ⟨u.val.succ, by simp⟩, by intro a b; simp; rw [Subtype.mk_eq_mk]; simp [Fin.val_inj]⟩ (by intro v; simp; unfold LT.lt IVar.instLT; simp only [OfNat.ofNat]; trans (3 + 1); rw [Nat.add_one_lt_add_one_iff]; exact v.prop; simp) []).addClause #[Literal.pos 1, Literal.neg 2]).addClause #[Literal.neg 1, Literal.pos 2]).addClause #[Literal.neg 10, Literal.pos 19]).cnf
 #eval (LawfulState.new ⟨5, by simp⟩ ⟨λ u : Fin 3 ↦ ⟨u.val.succ, by simp⟩, by intro a b; simp; rw [Subtype.mk_eq_mk]; simp [Fin.val_inj]⟩ (by intro v; simp; unfold LT.lt IVar.instLT; simp only [OfNat.ofNat]; trans (3 + 1); rw [Nat.add_one_lt_add_one_iff]; exact v.prop; simp) []).nextVar
+#check (LawfulState.new ⟨5, by simp⟩ ⟨λ u : Fin 3 ↦ ⟨u.val.succ, by simp⟩, by intro a b; simp; rw [Subtype.mk_eq_mk]; simp [Fin.val_inj]⟩ (by intro v; simp; unfold LT.lt IVar.instLT; simp only [OfNat.ofNat]; trans (3 + 1); rw [Nat.add_one_lt_add_one_iff]; exact v.prop; simp) []).withTemps (none : Option (Fin 5 → String))
 
 end Trestle.Encode.Cardinality
